Define recovery weakestpre.
Recovery weakest pre takes an expression and a recovery procedure to run in
case the expression crashes. It's defined as a guarded fixed point of repeated
crash weakest pres.

We then have a straight-forward proof of what Argosy calls the "idempotence"
lemma: to prove a recovery weakest pre, it suffices to prove appropriate
crash weakest pres for the expression and the recovery procedure.

This definition is not perfect yet I think, but the fact that we get this
resemblence to the Argosy stuff suggests to me that this is a better way to
phrase things.

src/program_logic/recovery_adequacy.v
@@ -2,13 +2,93 @@ From iris.proofmode Require Import tactics.
 From iris.algebra Require Import gmap auth agree gset coPset.
 From iris.base_logic.lib Require Import wsat.
 From iris.program_logic Require Export weakestpre.
-From Perennial.program_logic Require Export crash_lang.
+From Perennial.program_logic Require Export crash_lang crash_weakestpre.
 
-(* Weakest pre-condition with a crash invariant. *)
-Definition wp_crash `{!irisG Λ Σ} s E e Φ Φinv :=
-  (WP e @ s ; E {{ Φ }} ∗
-  (∀ σ κs n, state_interp σ κs n ={⊤,∅}=∗ Φinv σ))%I.
+Class pbundleG (T: ofeT) := {
+  pbundleT : T
+}.
 
+Class perennialG (Λ : language) (CS: crash_semantics Λ) (T: ofeT) (Σ : gFunctors) := IrisG {
+  perennial_irisG :> pbundleG T → irisG Λ Σ;
+}.
+
+Definition wpr_pre `{perennialG Λ CS T Σ} (s : stuckness)
+    (wpr : pbundleG T -d> coPset -d> expr Λ -d> expr Λ -d> (val Λ -d> iPropO Σ) -d> iPropO Σ -d> iPropO Σ) :
+  pbundleG T -d> coPset -d> expr Λ -d> expr Λ -d> (val Λ -d> iPropO Σ) -d> iPropO Σ -d> iPropO Σ :=
+  λ t E e rec Φ Φr,
+  (WPC e @ s ; E ; ∅
+     {{ Φ }}
+     {{ ∀ σ σ' (HC: crash_prim_step CS σ σ') κs n,
+        state_interp σ κs n ={∅}=∗  ▷ ∃ t, state_interp σ' [] 0 ∗ wpr t E rec rec (λ _, Φr) Φr }})%I.
+
+Local Instance wpr_pre_contractive `{!perennialG Λ CS T Σ} s : Contractive (wpr_pre s).
+Proof.
+  rewrite /wpr_pre=> n wp wp' Hwp t E1 e1 rec Φ Φc.
+  repeat (f_contractive || f_equiv); apply Hwp.
+Qed.
+
+Definition wpr_def `{!perennialG Λ CS T Σ} (s : stuckness) :
+  pbundleG T → coPset → expr Λ → expr Λ → (val Λ → iProp Σ) → iProp Σ → iProp Σ := fixpoint (wpr_pre s).
+Definition wpr_aux `{!perennialG Λ CS T Σ} : seal (@wpr_def Λ CS T Σ _). by eexists. Qed.
+Definition wpr `{!perennialG Λ CS T Σ} := wpr_aux.(unseal).
+Definition wpr_eq `{!perennialG Λ CS T Σ} : wpr = @wpr_def Λ CS T Σ _ := wpr_aux.(seal_eq).
+
+Section wpr.
+Context `{!perennialG Λ CS T Σ}.
+Implicit Types s : stuckness.
+Implicit Types P : iProp Σ.
+Implicit Types Φ : val Λ → iProp Σ.
+Implicit Types Φc : iProp Σ.
+Implicit Types v : val Λ.
+Implicit Types e : expr Λ.
+
+Lemma wpr_unfold s t E e rec Φ Φc :
+  wpr s t E e rec Φ Φc ⊣⊢ wpr_pre s (wpr s) t E e rec Φ Φc.
+Proof. rewrite wpr_eq. apply (fixpoint_unfold (wpr_pre s)). Qed.
+
+(* There's a stronger version of this *)
+Lemma wpr_strong_mono s t E e rec Φ Ψ Φr Ψr :
+  wpr s t E e rec Φ Φr -∗
+  (∀ v, Φ v ==∗ Ψ v) ∧ (Φr ==∗ Ψr) -∗
+  wpr s t E e rec Ψ Ψr.
+Proof.
+  iIntros "H HΦ". iLöb as "IH" forall (e t E Φ Ψ Φr Ψr).
+  rewrite ?wpr_unfold /wpr_pre.
+  iApply (wpc_strong_mono with "H") ; auto.
+  iSplit.
+  { iDestruct "HΦ" as "(H&_)". iIntros. iMod ("H" with "[$]"); eauto. }
+  iIntros "H". 
+  iModIntro. iIntros (?????) "Hinterp". iMod ("H" with "[//] Hinterp") as "H".
+  iModIntro. iNext. iDestruct "H" as (?) "(?&H)".
+  iExists _. iFrame. iApply ("IH" with "[$]").
+  iSplit; iIntros; iDestruct ("HΦ") as "(_&H)"; by iMod ("H" with "[$]").
+Qed.
+
+(* To prove a recovery wp for e with rec, it suffices to prove a crash wp for e, where the crash
+   condition implies the precondition for a crash wp for rec *)
+(* XXX the second predicate for wpr should take t as an argument, so we don't have this existential *)
+Lemma idempotence_wpr s E e rec Φx Φrx Φcx t:
+  ((WPC e @ s ; E ; ∅ {{ Φx t }} {{ Φcx t }}) -∗
+   (□ ∀ (t: pbundleG T) σ σ' (HC: crash_prim_step CS σ σ') κs n,
+        Φcx t -∗ state_interp σ κs n ={∅}=∗
+        ▷ ∃ t', state_interp σ' [] 0 ∗ WPC rec @ s ; E ; ∅ {{ (λ _, Φrx t') }} {{ Φcx t' }}) -∗
+    wpr s t E e rec (Φx t) (∃ t', Φrx t'))%I.
+Proof.
+  iLöb as "IH" forall (E e t Φx).
+  iIntros "He #Hidemp".
+  rewrite wpr_unfold. rewrite /wpr_pre.
+  iApply (wpc_strong_mono with "He"); [ auto | auto | auto | ].
+  iSplit; first auto. iIntros "Hcx". iModIntro.
+  iIntros. iMod ("Hidemp" with "[ ] [$] [$]") as "H".
+  { eauto. }
+  iModIntro. iNext. iDestruct "H" as (t') "(?&Hc)".
+  iExists _. iFrame.
+  iApply ("IH" $! E rec t' (λ t _, ∃ t', Φrx t')%I with "[Hc]").
+  { iApply (wpc_strong_mono with "Hc"); auto. }
+  eauto.
+Qed.
+
+(*
 Definition recv_idemp Σ {Λ CS} `{!invPreG Σ} s (rec: expr Λ) φinv φrec :=
   (□ (∀ `{Hinv : invG Σ} σ1 σ1' κs (Hcrash: crash_prim_step CS σ1 σ1'),
         (φinv σ1 ={⊤}=∗
@@ -17,3 +97,5 @@ Definition recv_idemp Σ {Λ CS} `{!invPreG Σ} s (rec: expr Λ) φinv φrec :=
              let _ : irisG Λ Σ := IrisG _ _ Hinv stateI fork_post in
              stateI σ1' κs 0 ∗
              wp_crash s ⊤ rec (λ _, ∀ σ n, stateI σ [] n ={⊤, ∅}=∗ φrec σ ) φinv)))%I.
+
+*)
